major update to extensions to eliminate the need to embed the whole external state in the extension corestate.  this makes the null_extension easier to define and easier to prove safe.

veric/extensions.v
@@ -1,366 +1,448 @@
 Load loadpath.
-Require Import veric.sim veric.step_lemmas veric.base veric.expr veric.extspec.
+Require Import msl.predicates_hered.
+Require Import veric.sim veric.step_lemmas veric.base veric.expr veric.extspec 
+               veric.juicy_extspec.
 Require Import ListSet.
 
 Set Implicit Arguments.
 
-Notation mem := Memory.mem.
+Lemma extfunct_eqdec : forall ef1 ef2 : AST.external_function, 
+  {ef1=ef2} + {~ef1=ef2}.
+Proof. intros ef1 ef2; repeat decide equality; apply Address.EqDec_int. Qed.
+
+Definition is_true (b: bool) := b=true.
+Local Coercion is_true: bool >-> Sortclass.
+
+Notation IN := (ListSet.set_mem extfunct_eqdec).
+Notation NOTIN := (fun ef l => ListSet.set_mem extfunct_eqdec ef l = false).
+Notation DIFF := (ListSet.set_diff extfunct_eqdec).
+
+Lemma in_diff (ef: AST.external_function) (l r: list AST.external_function) :
+  IN ef l -> NOTIN ef r -> IN ef (DIFF l r).
+Proof.
+simpl; intros H1 H2; apply set_mem_correct2. 
+apply set_mem_correct1 in H1.
+apply set_mem_complete1 in H2.
+apply set_diff_intro; auto.
+Qed.
+
+(*linking external specification "sigma" with an extension implementing
+   functions in "handled" corresponds to removing the functions in handled from
+   the external specification*)
+
+Definition link_ext_spec (M Z: Type) (handled: list AST.external_function) 
+  (sigma: external_specification M AST.external_function Z) :=
+  Build_external_specification M AST.external_function Z
+    (ext_spec_type sigma)
+    (fun (ef: AST.external_function) (x: ext_spec_type sigma ef)
+         (tys: list typ) (args: list val) (z: Z) (m: M) => 
+             if ListSet.set_mem extfunct_eqdec ef handled then False 
+             else ext_spec_pre sigma ef x tys args z m)
+    (fun (ef: AST.external_function) (x: ext_spec_type sigma ef)
+         (ty: option typ) (ret: option val) (z: Z) (m: M) => 
+             if ListSet.set_mem extfunct_eqdec ef handled then True
+             else ext_spec_post sigma ef x ty ret z m).
+
+Program Definition link_juicy_ext_spec (Z: Type) (handled: list AST.external_function)
+  (sigma: juicy_ext_spec Z) :=
+  Build_juicy_ext_spec Z (link_ext_spec handled sigma) _ _.
+Next Obligation.
+if_tac; [unfold hereditary; auto|].
+generalize JE_pre_hered; unfold hereditary; intros; eapply H; eauto.
+Qed.
+Next Obligation.
+if_tac; [unfold hereditary; auto|].
+generalize JE_post_hered; unfold hereditary; intros; eapply H; eauto.
+Qed.
+
+(*an external signature "ext_sig" is a list of handled functions together with
+   an external specification*)
 
 Section ExtSig.
-Variables (M ora_state: Type).
+Variables M Z: Type.
 
-Inductive extsig := mk_extsig: 
-  forall (handled: list AST.external_function)
-         (extspec: external_specification M external_function ora_state), 
-         extsig.
+Inductive ext_sig := 
+  mkextsig: forall (functs: list AST.external_function)
+                   (extspec: external_specification M external_function Z), 
+    ext_sig.
 
-Definition extsig2handled (sigma: extsig) :=
-  match sigma with mk_extsig l _ => l end.
-Coercion extsig2handled : extsig >-> list.
+Definition extsig2functs (sigma: ext_sig) := 
+  match sigma with mkextsig l _ => l end.
+Coercion extsig2functs : ext_sig >-> list.
 
-Definition extsig2extspec (sigma: extsig) :=
-  match sigma with mk_extsig _ spec => spec end.
-Coercion extsig2extspec : extsig >-> external_specification.
+Definition extsig2extspec (sigma: ext_sig) :=
+  match sigma with mkextsig functs spec => spec end.
+Coercion extsig2extspec : ext_sig >-> external_specification.
 
-Definition spec_of 
-  (ef: AST.external_function) (sigma: extsig) (x: ext_spec_type sigma ef) :=
-  (ext_spec_pre sigma ef x, ext_spec_post sigma ef x).
-
-Definition handles (ef: AST.external_function) (sigma: extsig) := 
-  List.In ef sigma.
+Definition spec_of (ef: AST.external_function) (sigma: ext_sig) :=
+  (ext_spec_pre sigma ef, ext_spec_post sigma ef).
 
 End ExtSig.
 
-(*for now, punt on spec extension (TO FILL IN LATER)*)
-Definition extends 
-  (M ora_state1 ora_state2: Type) 
-  (sigma1: extsig M ora_state1) (sigma2: extsig M ora_state2) :=
-  forall ef, List.In ef sigma1 -> List.In ef sigma2.
+Record juicy_ext_sig (Z: Type): Type := mkjuicyextsig {
+  JE_functs:> list external_function;
+  JE_extspec:> juicy_ext_spec Z
+}.
 
-Lemma extfunc_eqdec : forall ef1 ef2 : AST.external_function, 
-  {ef1=ef2} + {~ef1=ef2}.
-Proof.
-intros ef1 ef2; repeat decide equality.
-apply Address.EqDec_int.
-apply Address.EqDec_int.
-Qed.
+Definition juicy_extsig2extsig (Z: Type) (je: juicy_ext_sig Z) :=
+  mkextsig (JE_functs je) (JE_extspec je).
+Coercion juicy_extsig2extsig: juicy_ext_sig >-> ext_sig.
 
-Section linkable.
-Variables (M W ext_state: Type) (proj_ext_state : W -> ext_state).
+Definition link (T Z: Type) (esig: ext_sig T Z) 
+      (handled: list AST.external_function) :=
+  mkextsig handled (link_ext_spec handled esig).
 
-Definition linkable (signature: extsig M ext_state) (handled: extsig M W) :=
-  (forall ef, List.In ef handled -> List.In ef signature) /\
-  (*ef:{P}{Q} (handled spec) is a subtype of ef:{P'}{Q'} (assumed by client)*)
-  (forall ef x x' P Q P' Q', 
-    spec_of ef handled x = (P, Q) -> spec_of ef signature x' = (P', Q') -> 
-    (forall tys args w m, P' tys args (proj_ext_state w) m -> P tys args w m) /\
-    (forall ty ret w m, Q ty ret w m -> Q' ty ret (proj_ext_state w) m)).
+Definition juicy_link (Z: Type) (jesig: juicy_ext_sig Z) 
+      (handled: list AST.external_function) :=
+  mkjuicyextsig handled (link_juicy_ext_spec handled jesig).
 
-End linkable.
+(*ef:{P}{Q} (ext_sig spec) is a subtype of ef:{P'}{Q'} (spec. assumed by client)*)
+Definition linkable (M Z: Type) 
+      (handled: list AST.external_function) 
+      (client_sig: ext_sig M Z) (ext_sig: ext_sig M Z) := 
+  forall ef P Q P' Q', 
+    IN ef (DIFF client_sig handled) -> 
+    spec_of ef ext_sig = (P, Q) -> 
+    spec_of ef client_sig = (P', Q') -> 
+    forall x' tys args m z, P' x' tys args z m -> 
+      exists x, P x tys args z m /\
+      forall ty ret m' z', Q x ty ret z' m' -> Q' x' ty ret z' m'.
 
-Definition link
-  (M ora_state1 ora_state2: Type) 
-  (sigma1: extsig M ora_state1) (sigma2: extsig M ora_state2) :=
-  mk_extsig (ListSet.set_diff extfunc_eqdec sigma1 sigma2) sigma1.
+Module Extension. 
+Record Sig
+  (G: Type) (*global environments*)
+  (xT: Type) (*corestates of extended semantics*)
+  (cT: Type) (*corestates of core semantics*)
+  (M: Type) (*memories*)
+  (D: Type) (*initialization data*)
+  (Z Zint Zext: Type) 
 
-Module Extension. Record Sig
-  (G: Type) (*type of global environments*)
-  (W: Type) (*type of corestates of extended semantics*)
-  (C: Type) (*type of corestates of core semantics*)
-  (M: Type) (*type of memories*)
-  (D: Type) (*type of initialization data*)
-  (ext_state: Type) (*the type of _really_ external state*)
+  (esem: CoreSemantics G xT M D) (*extended semantics*)
+  (csem: nat -> option (CoreSemantics G cT M D)) (*a set of core semantics*)
 
-  (*extended semantics*)
-  (wsem: CoreSemantics G W M D) 
-  (*a set of core semantics*)
-  (csem: nat -> option (CoreSemantics G C M D))
+  (client_sig: ext_sig M Z) 
+  (esig: ext_sig M Z)
+  (handled: list AST.external_function) := Make {
 
-  (*signature of external functions*)
-  (signature: extsig M ext_state)
-  (*subset of external functions "implemented" by this extension*)
-  (handled: extsig M W) := Make {
+    (*generalized projection of core i from state s*)
+    proj_core : xT -> nat -> option cT;
+    core_exists : forall ge i s c' m s' m', 
+      corestep esem ge s m s' m' -> proj_core s' i = Some c' -> 
+      exists c, proj_core s i = Some c;
 
-    (*generalized projection of core i from state w*)
-    proj_core : W -> nat -> option C;
-    proj_exists : forall ge i w c' m w' m', 
-      corestep wsem ge w m w' m' -> proj_core w' i = Some c' -> 
-      exists c, proj_core w i = Some c;
+    (*the active (i.e., currently scheduled) core*)
+    active : xT -> nat;
+    active_csem : forall s, exists CS, csem (active s) = Some CS;
+    active_proj_core : forall s, exists c, proj_core s (active s) = Some c;
 
-    (*the active (i.e., currently scheduled) thread*)
-    active : W -> nat;
-    active_csem : forall w, exists CS, csem (active w) = Some CS;
-    active_proj_core : forall w, exists c, proj_core w (active w) = Some c;
-
-    (*runnable = Some i when active w = i and i is runnable (i.e., not blocked
+    (*runnable = Some i when active s = i and i is runnable (i.e., not blocked
       waiting on an external function call)*)
-    runnable : G -> W -> option nat;
-    runnable_active : forall ge w i, 
-      runnable ge w = Some i -> active w = i;
-    runnable_none : forall ge w c CS,
-      runnable ge w = None -> 
-      csem (active w) = Some CS -> proj_core w (active w) = Some c -> 
+    runnable : G -> xT -> option nat;
+    runnable_active : forall ge s i, 
+      runnable ge s = Some i -> active s = i;
+    runnable_none : forall ge s c CS,
+      runnable ge s = None -> 
+      csem (active s) = Some CS -> proj_core s (active s) = Some c -> 
       (exists rv, safely_halted CS ge c = Some rv) \/
       (exists ef, exists args, at_external CS c = Some (ef, args));
 
-    (*a thread is no longer "at external" once the extension has returned 
-      to it with the result of the external function call*)
+    (*a core is no longer "at external" once the extension has returned 
+      to it with the result of the call on which it was blocked*)
     after_at_external_excl : forall i CS c c' ret,
       csem i = Some CS -> after_external CS ret c = Some c' -> 
       at_external CS c' = None;
 
-    handles_ok: forall w i CS c ef args sig,
-      csem i = Some CS -> proj_core w i = Some c -> 
+    at_external_client_sig: forall s i CS c ef args sig,
+      csem i = Some CS -> proj_core s i = Some c -> 
       at_external CS c = Some (ef, sig, args) -> 
-      at_external wsem w = None -> 
-      handles ef signature;
+      IN ef client_sig;
+    notat_external_handled: forall s i CS c ef args sig,
+      csem i = Some CS -> proj_core s i = Some c -> 
+      at_external CS c = Some (ef, sig, args) -> 
+      at_external esem s = None -> 
+      IN ef handled;
+    at_external_not_handled: forall s ef args sig,
+      at_external esem s = Some (ef, sig, args) -> 
+      NOTIN ef handled;
 
-    (*type W embeds the external state*)
-    proj_ext_state : W -> ext_state;
-    lift_pred : (ext_state -> M -> Prop) -> (W -> M -> Prop);
-    proj_ext_state_pre : forall ef x P Q tys args w m,
-      spec_of ef (link signature handled) x = (P, Q) -> 
-      (P tys args (proj_ext_state w) m <-> lift_pred (P tys args) w m);
-    proj_ext_state_post : forall ef x P Q ty ret w m,
-      spec_of ef (link signature handled) x = (P, Q) -> 
-      (Q ty ret (proj_ext_state w) m <-> lift_pred (Q ty ret) w m);
-    ext_upd_at_external : forall ge w m w' m',
-      corestep wsem ge w m w' m' -> 
-      proj_ext_state w = proj_ext_state w';
+    (*type xT embeds Zint*)
+    proj_zint: xT -> Zint;
+    proj_zext: Z -> Zext;
+    zmult: Zint -> Zext -> Z;
+    zmult_proj: forall zint zext, proj_zext (zmult zint zext) = zext;
+    ext_upd_at_external : forall ge s m s' m',
+      corestep esem ge s m s' m' -> 
+      proj_zint s = proj_zint s';
 
-    (*generic injection of updated external state into a W*)
-    inj_ext_state : ext_state -> W -> W;
-    proj_inj : forall ora w, proj_ext_state (inj_ext_state ora w) = ora;
+    (*csem and esem are signature linkable*)
+    esem_csem_linkable: linkable handled client_sig esig;
 
-    (*csem and wsem are signature linkable*)
-    csem_wsem_linkable: linkable proj_ext_state signature handled;
-
-    (*a global invariant characterizing "safe" extensions: an projectible core 
-       is safeN*)
-    all_safe (ge: G) (n: nat) (w: W) (m: M) :=
+    (*a global invariant characterizing "safe" extensions*)
+    all_safe (ge: G) (n: nat) (z: Z) (w: xT) (m: M) :=
       forall i CS c, csem i = Some CS -> proj_core w i = Some c -> 
-        safeN CS signature ge n (proj_ext_state w) c m
-  }.
+        safeN CS client_sig ge n z c m
+}.
 
 End Extension. 
 
-Implicit Arguments Extension.Make [G W C M D ext_state].
+Implicit Arguments Extension.Make [G xT cT M D Z Zint Zext].
 
 (*an extension E is safe when all states satisfy the "all_safe" invariant*)
+
 Section SafeExtension.
-Variables
-  (G W C M D ext_state: Type) 
-  (wsem: CoreSemantics G W M D) 
-  (csem: nat -> option (CoreSemantics G C M D))
-  (signature: extsig M ext_state)
-  (handled: extsig M W).
+Variables (G T C M D Z Zint Zext: Type)
+  (esem: CoreSemantics G T M D) (csem: nat -> option (CoreSemantics G C M D))
+  (client_sig: ext_sig M Z) (esig: ext_sig M Z) (handled: list AST.external_function).
 
-Notation all_safe := Extension.all_safe.
+Import Extension.
 
-Definition safe_extension (E: Extension.Sig wsem csem signature handled) := 
-  forall ge n w m,  E.(all_safe) ge n w m -> 
-    safeN wsem (link signature handled) ge n (E.(Extension.proj_ext_state) w) w m.
+Definition safe_extension (E: Extension.Sig Zint Zext esem csem client_sig esig handled) :=
+  forall ge n s m z, 
+    E.(all_safe) ge n (zmult E (proj_zint E s) z) s m -> 
+    safeN esem (link esig handled) ge n (zmult E (proj_zint E s) z) s m.
 
 End SafeExtension.
 
 Section SafetyMonotonicity.
-Variables 
-  (G C W M D ext_state: Type) (CS: CoreSemantics G C M D)
-  (signature: extsig M ext_state) 
-  (handled: extsig M W).
+Variables (G cT M D Zext: Type) (CS: CoreSemantics G cT M D)
+  (client_sig: ext_sig M Z) (handled: ext_sig M Zext).
 
-(*this is somewhat vacuous now because of the defn. of linking*)
-Lemma safety_monotonicity : forall ge n ora c m,
-  safeN CS (link signature handled) ge n ora c m -> 
-  safeN CS signature ge n ora c m.
-Proof. intros ge n; induction n; simpl; auto. Qed.
+Lemma safety_monotonicity : forall ge n z c m,
+  safeN CS (link client_sig handled) ge n z c m -> 
+  safeN CS client_sig ge n z c m.
+Proof. 
+intros ge n; induction n; auto.
+intros  ora c m; simpl; intros H1.
+destruct (at_external CS c).
+destruct p; destruct p.
+destruct (safely_halted CS ge c).
+auto.
+destruct H1 as [x [H1 H2]].
+if_tac in H1.
+elimtype False; apply H1.
+exists x; split; auto.
+intros ret m' z' H3; destruct (H2 ret m' z' H3) as [c' [H4 H5]].
+exists c'; split; auto.
+destruct (safely_halted CS ge c); auto.
+destruct H1 as [c' [m' [H1 H2]]].
+exists c'; exists m'; split; auto.
+Qed.
 
 End SafetyMonotonicity.
 
 Section SafetyCriteria.
 Variables
-  (G W C M D ext_state: Type) 
-  (wsem: CoreSemantics G W M D) 
-  (csem: nat -> option (CoreSemantics G C M D))
-  (signature: extsig M ext_state)
-  (handled: extsig M W)
-  (E: Extension.Sig wsem csem signature handled).
+  (G xT cT M D Z Zint Zext: Type) 
+  (esem: CoreSemantics G xT M D) 
+  (csem: nat -> option (CoreSemantics G cT M D))
+  (client_sig: ext_sig M Z)
+  (esig: ext_sig M Z)
+  (handled: list AST.external_function)
+  (E: Extension.Sig Zint Zext esem csem client_sig esig handled).
+
+Definition proj_zint := E.(Extension.proj_zint). 
+Local Coercion proj_zint : xT >-> Zint.
+
+Definition proj_zext := E.(Extension.proj_zext).
+Local Coercion proj_zext : Z >-> Zext.
 
 Notation ALL_SAFE := E.(Extension.all_safe).
-Notation PROJ := E.(Extension.proj_core).
-Notation PROJ_EXT := E.(Extension.proj_ext_state).
-Notation INJ_EXT := E.(Extension.inj_ext_state).
-Notation LIFT := E.(Extension.lift_pred).
+Notation PROJ_CORE := E.(Extension.proj_core).
+Notation "zint \o zext" := (E.(Extension.zmult) zint zext) (at level 66, left associativity). 
 Notation ACTIVE := (E.(Extension.active)).
 Notation RUNNABLE := (E.(Extension.runnable)).
-Notation "'THREAD' i 'is' ( CS , c ) 'in' w" := 
-  (csem i = Some CS /\ PROJ w i = Some c)
+Notation "'CORE' i 'is' ( CS , c ) 'in' s" := 
+  (csem i = Some CS /\ PROJ_CORE s i = Some c)
   (at level 66, no associativity, only parsing).
-Notation proj_exists := E.(Extension.proj_exists).
+Notation core_exists := E.(Extension.core_exists).
 Notation active_csem := E.(Extension.active_csem).
 Notation active_proj_core := E.(Extension.active_proj_core).
 Notation after_at_external_excl := E.(Extension.after_at_external_excl).
-Notation handles_ok := E.(Extension.handles_ok).
-Notation proj_inj := E.(Extension.proj_inj).
-Notation proj_ext_state_pre := E.(Extension.proj_ext_state_pre).
-Notation proj_ext_state_post := E.(Extension.proj_ext_state_post).
+Notation notat_external_handled := E.(Extension.notat_external_handled).
+Notation at_external_not_handled := E.(Extension.at_external_not_handled).
 Notation ext_upd_at_external := E.(Extension.ext_upd_at_external).
 Notation runnable_active := E.(Extension.runnable_active).
 Notation runnable_none := E.(Extension.runnable_none).
 
-Lemma all_safe_downward ge n w m :
-  ALL_SAFE ge (S n) w m -> ALL_SAFE ge n w m.
+Lemma all_safe_downward ge n z s m :
+  ALL_SAFE ge (S n) z s m -> ALL_SAFE ge n z s m.
 Proof. intros INV i CS c H2 H3; eapply safe_downward1; eauto. Qed.
 
 Inductive safety_criteria: Type := SafetyCriteria: forall 
   (*coresteps preserve the invariant*)
-  (core_pres: forall ge n w c m CS i w' c' m', 
-    ALL_SAFE ge (S n) w m -> 
-    ACTIVE w = i -> THREAD i is (CS, c) in w -> 
-    corestep CS ge c m c' m' -> corestep wsem ge w m w' m' -> 
-    THREAD i is (CS, c') in w' /\ ALL_SAFE ge n w' m')
+  (core_pres: forall ge n z (s: xT) c m CS i s' c' m', 
+    ALL_SAFE ge (S n) (s \o z) s m -> 
+    ACTIVE s = i -> CORE i is (CS, c) in s -> 
+    corestep CS ge c m c' m' -> corestep esem ge s m s' m' -> 
+    CORE i is (CS, c') in s' /\ ALL_SAFE ge n (s' \o z) s' m')
 
   (*corestates satisfying the invariant can corestep*)
-  (core_prog: forall ge n w m i c CS, 
-    ALL_SAFE ge (S n) w m -> 
-    ACTIVE w = i -> RUNNABLE ge w = Some i -> THREAD i is (CS, c) in w -> 
-    exists c', exists w', exists m', 
-      corestep CS ge c m c' m' /\ corestep wsem ge w m w' m' /\
-      THREAD i is (CS, c') in w')
+  (core_prog: forall ge n z s m i c CS, 
+    ALL_SAFE ge (S n) z s m -> 
+    ACTIVE s = i -> RUNNABLE ge s = Some i -> CORE i is (CS, c) in s -> 
+    exists c', exists s', exists m', 
+      corestep CS ge c m c' m' /\ corestep esem ge s m s' m' /\
+      CORE i is (CS, c') in s')
 
   (*"handled" steps respect function specifications*)
-  (handled_pres: forall ge w m c w' m' c' CS ef sig args P Q x, 
-    let i := ACTIVE w in THREAD i is (CS, c) in w -> 
+  (handled_pres: forall ge s z m c s' m' c' CS ef sig args P Q x, 
+    let i := ACTIVE s in CORE i is (CS, c) in s -> 
     at_external CS c = Some (ef, sig, args) -> 
-    handles ef signature -> 
-    spec_of ef signature x = (P, Q) -> LIFT (P (sig_args sig) args) w m -> 
-    corestep wsem ge w m w' m' -> 
-    THREAD i is (CS, c') in w' -> 
-      ((at_external CS c' = Some (ef, sig, args) /\ LIFT (P (sig_args sig) args) w' m' /\
-        (forall j, ACTIVE w' = j -> i <> j)) \/
-      (exists ret, after_external CS ret c = Some c' /\ LIFT (Q (sig_res sig) ret) w' m')))
+    ListSet.set_mem extfunct_eqdec ef handled = true -> 
+    spec_of ef client_sig = (P, Q) -> 
+    P x (sig_args sig) args (s \o z) m -> 
+    corestep esem ge s m s' m' -> 
+    CORE i is (CS, c') in s' -> 
+      ((at_external CS c' = Some (ef, sig, args) /\ P x (sig_args sig) args (s' \o z) m' /\
+        (forall j, ACTIVE s' = j -> i <> j)) \/
+      (exists ret, after_external CS ret c = Some c' /\ Q x (sig_res sig) ret (s' \o z) m')))
 
-  (*"handled" states satisfying the invariant can step or are safely halted; 
+  (*"handled" states satisfying the invariant can step or are safely halted;
      core states that stay "at_external" remain unchanged*)
-  (handled_prog: forall ge n w m,
-    ALL_SAFE ge n w m -> RUNNABLE ge w = None -> 
-    at_external wsem w = None -> 
-    (exists w', exists m', corestep wsem ge w m w' m' /\ 
-      forall i c CS, THREAD i is (CS, c) in w -> 
-        exists c', THREAD i is (CS, c') in w' /\ 
+
+  (handled_prog: forall ge n z s m,
+    ALL_SAFE ge n z s m -> RUNNABLE ge s = None -> 
+    at_external esem s = None -> 
+    (exists s', exists m', corestep esem ge s m s' m' /\ 
+      forall i c CS, CORE i is (CS, c) in s -> 
+        exists c', CORE i is (CS, c') in s' /\ 
           (forall ef args ef' args', 
             at_external CS c = Some (ef, args) -> 
             at_external CS c' = Some (ef', args') -> c=c')) \/
-    (exists rv, safely_halted wsem ge w = Some rv))
+    (exists rv, safely_halted esem ge s = Some rv))
 
   (*safely halted threads remain halted*)
-  (safely_halted_halted: forall ge w m w' m' i CS c rv,
-    THREAD i is (CS, c) in w -> safely_halted CS ge c = Some rv -> 
-    corestep wsem ge w m w' m' -> 
-    THREAD i is (CS, c) in w')
+  (safely_halted_halted: forall ge s m s' m' i CS c rv,
+    CORE i is (CS, c) in s -> safely_halted CS ge c = Some rv -> 
+    corestep esem ge s m s' m' -> 
+    CORE i is (CS, c) in s')
 
-  (*safety of other threads is preserved when handling one step of 
-     blocked thread i*)
-  (handled_rest: forall ge w m w' m' c CS,
-    let i := ACTIVE w in THREAD i is (CS, c) in w -> 
+  (*safety of other threads is preserved when handling one step of blocked
+     thread i*)
+ 
+ (handled_rest: forall ge s m s' m' c CS,
+    let i := ACTIVE s in CORE i is (CS, c) in s -> 
     ((exists ef, exists args, at_external CS c = Some (ef, args)) \/ 
       exists rv, safely_halted CS ge c = Some rv) -> 
-    at_external wsem w = None -> 
-    corestep wsem ge w m w' m' -> 
+    at_external esem s = None -> 
+    corestep esem ge s m s' m' -> 
     (forall CS0 c0 j, i <> j ->  
-      (THREAD j is (CS0, c0) in w' -> THREAD j is (CS0, c0) in w) /\
-      (forall n, THREAD j is (CS0, c0) in w -> 
-                 safeN CS0 signature ge (S n) (PROJ_EXT w) c0 m -> 
-                 safeN CS0 signature ge n (PROJ_EXT w') c0 m')))
+      (CORE j is (CS0, c0) in s' -> CORE j is (CS0, c0) in s) /\
+      (forall n z z', CORE j is (CS0, c0) in s -> 
+                      safeN CS0 client_sig ge (S n) (s \o z) c0 m -> 
+                      safeN CS0 client_sig ge n (s' \o z') c0 m')))
 
-  (*if the extended machine is at external, then the active thread is
-     at external (an extension only implements external functions, it doesn't
+  (*if the extended machine is at external, then the active thread is at
+     external (an extension only implements external functions, it doesn't
      introduce them)*)
-  (at_extern_call: forall w ef args,
-    at_external wsem w = Some (ef, args) -> 
+
+  (at_extern_call: forall s ef sig args,
+    at_external esem s = Some (ef, sig, args) -> 
     exists CS, exists c, 
-      THREAD (ACTIVE w) is (CS, c) in w /\ 
-      at_external CS c = Some (ef, args))
+      CORE (ACTIVE s) is (CS, c) in s /\ 
+      at_external CS c = Some (ef, sig, args))
 
   (*inject the results of an external call into the extended machine state*)
-  (at_extern_ret: forall c w m ora m' tys args ty ret c' P Q CS ef x,
-    let i := ACTIVE w in THREAD i is (CS, c) in w -> 
-    spec_of ef signature x = (P, Q) -> 
-    P tys args (PROJ_EXT w) m -> Q ty ret ora m' -> 
+  (at_extern_ret: forall c z s m z' m' tys args ty ret c' CS ef sig x 
+      (P:ext_spec_type esig ef -> list typ -> list val -> Z -> M -> Prop) 
+      (Q: ext_spec_type esig ef -> option typ -> option val -> Z -> M -> Prop),
+    let i := ACTIVE s in CORE i is (CS, c) in s -> 
+    at_external esem s = Some (ef, sig, args) -> 
+    spec_of ef esig = (P, Q) -> 
+    P x tys args (s \o z) m -> Q x ty ret z' m' -> 
     after_external CS ret c = Some c' -> 
-    exists w', 
-      INJ_EXT ora w' = w' /\
-      after_external wsem ret w = Some w' /\ 
-      THREAD i is (CS, c') in w') 
+    exists s': xT, 
+      z' = s' \o z' /\
+      after_external esem ret s = Some s' /\ 
+      CORE i is (CS, c') in s')
 
   (*safety of other threads is preserved when returning from an external 
      function call*)
-  (at_extern_rest: forall c w m ora w' m' tys args ty ret c' P Q CS ef x,
-    let i := ACTIVE w in THREAD i is (CS, c) in w -> 
-    spec_of ef signature x = (P, Q) -> 
-    P args tys (PROJ_EXT w) m -> Q ty ret ora m' -> 
+  (at_extern_rest: forall c z s m z' s' m' tys args ty ret c' CS ef x sig
+      (P:ext_spec_type esig ef -> list typ -> list val -> Z -> M -> Prop) 
+      (Q: ext_spec_type esig ef -> option typ -> option val -> Z -> M -> Prop),
+    let i := ACTIVE s in CORE i is (CS, c) in s -> 
+    at_external esem s = Some (ef, sig, args) -> 
+    spec_of ef esig = (P, Q) -> 
+    P x tys args (s \o z) m -> Q x ty ret z' m' -> 
     after_external CS ret c = Some c' -> 
-    after_external wsem ret w = Some w' -> 
-    THREAD i is (CS, c') in w' -> 
+    after_external esem ret s = Some s' -> 
+    CORE i is (CS, c') in s' -> 
     (forall CS0 c0 j, i <> j -> 
-      (THREAD j is (CS0, c0) in w' -> THREAD j is (CS0, c0) in w) /\
-      (forall ge n, THREAD j is (CS0, c0) in w -> 
-                    safeN CS0 signature ge (S n) (PROJ_EXT w) c0 m -> 
-                    safeN CS0 signature ge n (PROJ_EXT w') c0 m'))),
+      (CORE j is (CS0, c0) in s' -> CORE j is (CS0, c0) in s) /\
+      (forall ge n, CORE j is (CS0, c0) in s -> 
+                    safeN CS0 client_sig ge (S n) (s \o z) c0 m -> 
+                    safeN CS0 client_sig ge n z' c0 m'))),
   safety_criteria.
 
 Lemma safety_criteria_safe : safety_criteria -> safe_extension E.
 Proof.
 inversion 1; subst; intros ge n; induction n.
-intros w m H1; simpl; auto.
-intros w m H1.
-simpl; case_eq (at_external wsem w).
+intros s m z H1; simpl; auto.
+intros s m z H1.
+simpl; case_eq (at_external esem s).
 
 (*CASE 1: at_external OUTER = Some _; i.e. _really_ at_external*) 
-intros [ef args] AT_EXT.
-destruct (at_external_halted_excl wsem ge w) as [H2|H2].
+intros [[ef sig] args] AT_EXT.
+destruct (at_external_halted_excl esem ge s) as [H2|H2].
 rewrite AT_EXT in H2; congruence.
 simpl; rewrite H2.
-destruct (at_extern_call w ef args AT_EXT) as [CS [c [[H3 H4] H5]]].
+destruct (at_extern_call s ef sig args AT_EXT) as [CS [c [[H3 H4] H5]]].
 generalize H1 as H1'; intro.
-specialize (H1 (ACTIVE w) CS c H3 H4).
+specialize (H1 (ACTIVE s) CS c H3 H4).
 simpl in H1.
 rewrite H5 in H1.
-destruct ef as [ef sig].
 destruct (at_external_halted_excl CS ge c) as [H6|H6].
 rewrite H6 in H5; congruence.
 rewrite H6 in H1; clear H6.
 destruct H1 as [x H1].
 destruct H1 as [H7 H8].
-exists x.
+generalize (Extension.esem_csem_linkable E); intros Hlink.
+assert (H16: IN ef (DIFF client_sig handled)).
+ apply in_diff.
+ eapply Extension.at_external_client_sig; eauto.
+ eapply Extension.at_external_not_handled; eauto.
+ auto.
+specialize (Hlink ef 
+  (ext_spec_pre esig ef) (ext_spec_post esig ef) 
+  (ext_spec_pre client_sig ef) (ext_spec_post client_sig ef) H16).
+destruct Hlink with (x' := x) 
+ (tys := sig_args sig) (args := args) (m := m) (z := (s \o z)) 
+ as [x' [H17 H18]]; auto.
+exists x'.
+erewrite at_external_not_handled; eauto.
 split; auto.
+erewrite at_external_not_handled; eauto.
 intros ret m' z' POST.
-destruct (H8 ret m' z' POST) as [c' [H10 H11]].
-specialize (at_extern_ret c w m z' m' (sig_args sig) args (sig_res sig) ret c' 
-  (ext_spec_pre signature ef x) (ext_spec_post signature ef x) CS ef x).
+destruct (H8 ret m' z') as [c' [H10 H11]].
+eapply H18 in POST; eauto.
+specialize (at_extern_ret c z s m z' m' (sig_args sig) args (sig_res sig) ret c' CS
+ ef sig x' (ext_spec_pre esig ef) (ext_spec_post esig ef)).
 hnf in at_extern_ret.
 spec at_extern_ret; auto.
 spec at_extern_ret; auto.
 spec at_extern_ret; auto.
 spec at_extern_ret; auto.
 spec at_extern_ret; auto.
-destruct at_extern_ret as [w' [H12 [H13 [H14 H15]]]].
-exists w'.
+spec at_extern_ret; auto.
+destruct at_extern_ret as [s' [H12 [H13 [H14 H15]]]].
+exists s'.
 split; auto.
-eapply safety_monotonicity.
-assert (z' = PROJ_EXT w') as -> by (rewrite <-H12, proj_inj; auto).
+rewrite H12.
 eapply IHn.
 intros j CSj cj CSEMJ PROJJ.
-case_eq (eq_nat_dec (ACTIVE w) j).
+case_eq (eq_nat_dec (ACTIVE s) j).
 (*i=j*)
 intros Heq _; rewrite Heq in *.
-rewrite CSEMJ in H14; inversion H14; rewrite H6 in *.
-rewrite PROJJ in H15; inversion H15; rewrite H9 in *.
+rewrite CSEMJ in H14; inversion H14; rewrite H1 in *.
+rewrite PROJJ in H15; inversion H15; rewrite H6 in *.
+unfold proj_zint in H12.
+rewrite <-H12.
 auto.
 (*i<>j*)
 intros Hneq _.
-specialize (at_extern_rest c w m (PROJ_EXT w') w' m' args (sig_args sig) (sig_res sig) ret c'
-  (ext_spec_pre signature ef x) (ext_spec_post signature ef x) CS ef x).
+specialize (at_extern_rest c z s m z' s' m' (sig_args sig) args (sig_res sig) ret c' CS
+  ef x' sig (ext_spec_pre esig ef) (ext_spec_post esig ef)).
 hnf in at_extern_rest.
 spec at_extern_rest; auto.
 spec at_extern_rest; auto.
@@ -369,75 +451,82 @@ spec at_extern_rest; auto.
 spec at_extern_rest; auto.
 spec at_extern_rest; auto.
 spec at_extern_rest; auto.
-destruct (at_extern_rest CSj cj j Hneq) as [H16 H17].
-eapply H17; eauto.
-destruct H16 as [H18 H19]; auto.
+spec at_extern_rest; auto.
+destruct (at_extern_rest CSj cj j Hneq) as [H19 H20].
+unfold proj_zint in H12.
+rewrite <-H12.
+eapply H20; eauto.
+destruct H19 as [H21 H22]; auto.
 eapply H1'; eauto.
 
 (*CASE 2: at_external OUTER = None; i.e., handled function*)
 intros H2.
-case_eq (safely_halted wsem ge w); auto.
-case_eq (RUNNABLE ge w).
+case_eq (safely_halted esem ge s); auto.
+case_eq (RUNNABLE ge s).
 (*active thread i*)
 intros i RUN.
 generalize (runnable_active _ _ RUN) as ACT; intro.
 rewrite <-ACT in *.
-destruct (active_csem w) as [CS CSEM].
-destruct (active_proj_core w) as [c PROJECT].
-destruct (core_prog ge n w m i c CS H1 ACT) 
- as [c' [w' [m' [CORESTEP_C [CORESTEP_W [CSEM' PROJECT']]]]]]; auto.
+destruct (active_csem s) as [CS CSEM].
+destruct (active_proj_core s) as [c PROJECT].
+destruct (core_prog ge n (s \o z) s m i c CS H1 ACT) 
+ as [c' [s' [m' [CORESTEP_C [CORESTEP_T [CSEM' PROJECT']]]]]]; auto.
 rewrite <-ACT; auto.
 rewrite <-ACT; auto.
-destruct (core_pres ge n w c m CS i w' c' m' H1 ACT)
+destruct (core_pres ge n z s c m CS i s' c' m' H1 ACT)
  as [_ INV']; auto.
 rewrite <-ACT in *; auto.
-exists w'; exists m'; split; [auto|].
-erewrite ext_upd_at_external; eauto.
+exists s'; exists m'; split; [auto|].
+apply ext_upd_at_external in CORESTEP_T.
+rewrite CORESTEP_T.
+eauto.
+
 (*no runnable thread*)
 intros RUN.
-destruct (active_csem w) as [CS CSEM].
-destruct (active_proj_core w) as [c PROJECT].
-destruct (handled_prog ge n w m (all_safe_downward H1) RUN H2)
- as [[w' [m' [CORESTEP_W CORES_PRES]]]|[rv SAFELY_HALTED]].
+destruct (active_csem s) as [CS CSEM].
+destruct (active_proj_core s) as [c PROJECT].
+destruct (handled_prog ge n (s \o z) s m (all_safe_downward H1) RUN H2)
+ as [[s' [m' [CORESTEP_T CORES_PRES]]]|[rv SAFELY_HALTED]].
 2: intros CONTRA; rewrite CONTRA in SAFELY_HALTED; congruence.
-exists w'; exists m'.
+exists s'; exists m'.
 split; auto.
 erewrite ext_upd_at_external; eauto; eapply IHn.
-destruct (runnable_none ge w RUN CSEM PROJECT) 
+destruct (runnable_none ge s RUN CSEM PROJECT) 
  as [SAFELY_HALTED|[ef [args AT_EXT]]].
 
 (*subcase A of no runnable thread: safely halted*)
 intros j CSj cj CSEMj PROJECTj.
-set (i := ACTIVE w) in *.
+set (i := ACTIVE s) in *.
 case_eq (eq_nat_dec i j).
 (*i=j*)
 intros Heq _; rewrite Heq in *.
-destruct (proj_exists ge j w m w' m' CORESTEP_W PROJECTj)
+destruct (core_exists ge j s m s' m' CORESTEP_T PROJECTj)
  as [c0 PROJECT0].
 rewrite PROJECT in PROJECT0; inversion PROJECT0; subst.
 rewrite CSEM in CSEMj; inversion CSEMj; rename H4 into H3; rewrite <-H3 in *.
 specialize (H1 j CS c0 CSEM PROJECT).
 simpl in H1. 
 destruct SAFELY_HALTED as [rv SAFELY_HALTED].
-destruct (@at_external_halted_excl G C M D CS ge c0) as [H4|H4]; 
+destruct (@at_external_halted_excl G cT M D CS ge c0) as [H4|H4]; 
  [|congruence].
 destruct n; simpl; auto.
-destruct (safely_halted_halted ge w m w' m' j CS c0 rv) as [H6 H7]; auto.
+destruct (safely_halted_halted ge s m s' m' j CS c0 rv) as [H6 H7]; auto.
 rewrite H7 in PROJECTj; inversion PROJECTj; subst.
 rewrite H4, SAFELY_HALTED; auto.
 (*i<>j*)
 intros Hneq _.
 destruct (CORES_PRES i c CS) as [c' [[_ PROJ'] H5]]. 
 split; auto.
-specialize (handled_rest ge w m w' m' c CS).
+specialize (handled_rest ge s m s' m' c CS).
 hnf in handled_rest.
 spec handled_rest; auto.
 spec handled_rest; auto.
 spec handled_rest; auto.
 spec handled_rest; auto.
 destruct (handled_rest CSj cj j Hneq) as [H6 H7].
-eapply H7; eauto.
-destruct (proj_exists ge j w m w' m' CORESTEP_W PROJECTj)
+eapply H7 with (z:=z); eauto.
+eapply H1; eauto.
+destruct (core_exists ge j s m s' m' CORESTEP_T PROJECTj)
  as [c0 PROJECT0].
 specialize (H1 j CSj c0 CSEMj PROJECT0).
 destruct H6 as [H8 H9].
@@ -446,13 +535,14 @@ rewrite H9 in PROJECT0; inversion PROJECT0; subst; auto.
 
 (*subcase B of no runnable thread: at external INNER*)
 intros j CSj cj CSEMj PROJECTj.
-set (i := ACTIVE w) in *.
+set (i := ACTIVE s) in *.
 case_eq (eq_nat_dec i j).
 (*i=j*)
 intros Heq _; rewrite Heq in *.
-destruct (proj_exists ge j w m w' m' CORESTEP_W PROJECTj)
+destruct (core_exists ge j s m s' m' CORESTEP_T PROJECTj)
  as [c0 PROJECT0].
 rewrite PROJECT in PROJECT0; inversion PROJECT0; subst.
+generalize CSEMj as CSEMj'; intro.
 rewrite CSEM in CSEMj; inversion CSEMj; rename H4 into H3; rewrite <-H3 in *.
 specialize (H1 j CS c0 CSEM PROJECT).
 simpl in H1. 
@@ -463,19 +553,17 @@ solve[destruct ef; elimtype False; auto].
 destruct ef as [ef sig].
 destruct H1 as [x H1].
 destruct H1 as [PRE POST].
-specialize (handled_pres ge w m c0 w' m' cj CS ef sig args
-  (ext_spec_pre signature ef x)
-  (ext_spec_post signature ef x) x).
+specialize (handled_pres ge s z m c0 s' m' cj CS ef sig args
+  (ext_spec_pre client_sig ef)
+  (ext_spec_post client_sig ef) x).
 rewrite Heq in handled_pres.
 hnf in handled_pres.
 spec handled_pres; auto.
 spec handled_pres; auto.
 spec handled_pres; auto. 
- eapply handles_ok; eauto.
+ eapply notat_external_handled; eauto.
 spec handled_pres; auto.
 spec handled_pres; auto.
-rewrite <-proj_ext_state_pre 
- with (ef := ef) (x := x) (Q := ext_spec_post signature ef x); auto.
 spec handled_pres; auto.
 spec handled_pres; auto.
 destruct (CORES_PRES j c0 CS) as [c' H4]; [split; auto|].
@@ -484,15 +572,13 @@ destruct handled_pres as [[AT_EXT' [PRE' ACT']] | POST'].
 destruct H4 as [[H4 H5] H6].
 rewrite H5 in PROJECTj; inversion PROJECTj; subst.
 specialize (H6 (ef,sig) args (ef,sig) args AT_EXT AT_EXT'); subst.
-clear - PRE' POST AT_EXT' H4 H5 HeqSAFELY_HALTED.
+clear - PRE' POST AT_EXT' H4 H5 HeqSAFELY_HALTED H2 AT_EXT PROJECT CSEMj'.
 destruct n; simpl; auto.
 rewrite AT_EXT', <-HeqSAFELY_HALTED.
 exists x.
-split.
-apply proj_ext_state_pre 
- with (ef := ef) (x := x) (Q := ext_spec_post signature ef x); auto.
-intros ret m'' w'' H8.
-destruct (POST ret m'' w'' H8) as [c'' [H9 H10]].
+split; auto.
+intros ret m'' s'' H8.
+destruct (POST ret m'' s'' H8) as [c'' [H9 H10]].
 exists c''; split; auto.
 eapply safe_downward1; eauto.
 (*post case*)
@@ -504,9 +590,7 @@ clear - PRE POST POST' AT_EXT' AFTER_EXT H4 H5 H6 HeqSAFELY_HALTED.
 destruct n; simpl; auto.
 rewrite AT_EXT'.
 case_eq (safely_halted CS ge c'); auto.
-apply proj_ext_state_post 
- with (ef := ef) (x := x) (P := ext_spec_pre signature ef x) in POST'; auto.
-destruct (POST ret m' (PROJ_EXT w') POST') as [c'' [AFTER_EXT' SAFEN]].
+destruct (POST ret m' (s' \o z) POST') as [c'' [AFTER_EXT' SAFEN]].
 rewrite AFTER_EXT in AFTER_EXT'; inversion AFTER_EXT'; subst.
 simpl in SAFEN.
 rewrite AT_EXT' in SAFEN.
@@ -517,7 +601,7 @@ exists c3; exists m''; split; auto.
 intros Hneq _.
 destruct (CORES_PRES i c CS) as [c' [[_ PROJ'] H5]]. 
 split; auto.
-specialize (handled_rest ge w m w' m' c CS).
+specialize (handled_rest ge s m s' m' c CS).
 hnf in handled_rest.
 spec handled_rest; auto.
 spec handled_rest; auto.
@@ -525,8 +609,9 @@ left; exists ef; exists args; auto.
 spec handled_rest; auto.
 spec handled_rest; auto.
 destruct (handled_rest CSj cj j Hneq) as [H6 H7].
-eapply H7; eauto.
-destruct (proj_exists ge j w m w' m' CORESTEP_W PROJECTj)
+eapply H7 with (z:=z); eauto.
+eapply H1; eauto.
+destruct (core_exists ge j s m s' m' CORESTEP_T PROJECTj)
  as [c0 PROJECT0].
 specialize (H1 j CSj c0 CSEMj PROJECT0).
 destruct H6 as [H8 H9].
