veric/null_extension.v
@@ -6,126 +6,86 @@ Require Import msl.base
 Set Implicit Arguments.
 
 Section NullExtSpec.
-Variables (M ext_state: Type) (ext_spec_type: AST.external_function -> Type).
+Variables (M Z: Type) (ext_spec_type: AST.external_function -> Type).
 
 Definition null_extspec := Build_external_specification 
-  M AST.external_function ext_state
+  M AST.external_function Z
   ext_spec_type
   (fun (ef: AST.external_function) (_:ext_spec_type ef) 
-       (tys: list typ) (args: list val) (z: ext_state) (m: M) => False)
+       (tys: list typ) (args: list val) (z: Z) (m: M) => False)
   (fun (ef: AST.external_function) (_:ext_spec_type ef) 
-       (ty: option typ) (ret: option val) (z: ext_state) (m: M) => True).
+       (ty: option typ) (ret: option val) (z: Z) (m: M) => True).
 
 End NullExtSpec.
 
 Section NullExtsig.
-Variable (M ext_state: Type) (ext_spec_type: AST.external_function -> Type).
+Variable (M Z: Type) (ext_spec_type: AST.external_function -> Type).
 
-Definition null_extsig := mk_extsig nil (null_extspec M ext_state ext_spec_type).
+Definition null_extsig := mkextsig nil (null_extspec M Z ext_spec_type).
 
 End NullExtsig.
 
 Section NullExtension.
 Variables 
-  (G C M D ext_state: Type) 
-  (csem: CoreSemantics G C M D)
-  (signature: extsig M ext_state)
-  (init_world: ext_state)
+  (G cT M D Z: Type) 
+  (csem: CoreSemantics G cT M D)
+  (client_sig: ext_sig M Z)
+  (init_world: Z)
 
   (after_at_external_excl: forall c ret c',
     after_external csem ret c = Some c' -> at_external csem c' = None)
   (at_external_handled: forall c ef args sig,
-    at_external csem c = Some (ef, sig, args) -> handles ef signature).
+    at_external csem c = Some (ef, sig, args) -> IN ef client_sig = true).
 
 Definition cores := fun _:nat => Some csem.
 
-Definition extension_state := (ext_state*C)%type.
-
-Program Definition wsem: CoreSemantics G extension_state M D := 
-  Build_CoreSemantics G extension_state M D 
-  (initial_mem csem)
-  (fun ge f args => match make_initial_core csem ge f args with
-                    | None => None
-                    | Some c => Some (init_world, c)
-                    end)
-  (at_external csem oo snd)
-  (fun ret s => match after_external csem ret (snd s) with 
-                | None => None
-                | Some c => Some (fst s, c)
-                end)
-  (fun ge s => safely_halted csem ge (snd s))
-  (fun ge s m s' m' => corestep csem ge (snd s) m (snd s') m' /\ fst s=fst s')
-  _ _ _.
-Next Obligation.
-destruct q; destruct q'; unfold compose; simpl in *.
-eapply corestep_not_at_external; eauto.
-Qed.
-Next Obligation.
-destruct q; destruct q'; simpl in *.
-eapply corestep_not_halted; eauto.
-Qed.
-Next Obligation.
-destruct q; unfold compose; simpl in *.
-eapply at_external_halted_excl.
-Qed.
-
 Local Open Scope nat_scope.
- 
-Definition proj_core (s: extension_state) (i:nat) := 
-  if eq_nat_dec i 1 then Some (snd s) else None.
-Definition active := fun _:extension_state => 1.
-Definition runnable := fun (ge: G) (s :extension_state) => 
-  match at_external csem (snd s), safely_halted csem ge (snd s) with 
+
+Definition proj_core (c: cT) (i: nat) := if eq_nat_dec i 1 then Some c else None.
+Definition active := fun _: cT => 1.
+Definition runnable := fun (ge: G) (s: cT) => 
+  match at_external csem s, safely_halted csem ge s with 
   | None, None => Some 1
   | _, _ => None
   end.
-Definition proj_ext_state := @fst ext_state C.
-Definition lift_pred (P: ext_state -> M -> Prop) := 
-  fun p:extension_state => P (fst p).
-Definition inj_ext_state (z: ext_state) (s: extension_state) := 
-  (z, snd s).
+Definition proj_zint := fun _: cT => tt.
+Definition proj_zext := fun z: Z => z.
+Definition zmult := fun (_: unit) (z: Z) => z.
+Definition handled: list AST.external_function := nil.
 
-(*Users will typically have to prove that their extension and client signatures
-   are compatible; here, we assume it since we are parametric in signature*)
-Variable null_extsig_linkable: forall S, 
-  linkable proj_ext_state S (null_extsig M (ext_state*C) 
-    (ext_spec_type signature)).
-
-Local Hint Unfold cores proj_core active runnable proj_ext_state 
-  lift_pred inj_ext_state : null_unfold.
+Local Hint Unfold cores proj_core active runnable proj_zint : null_unfold.
 
 Obligation Tactic := 
   autounfold with null_unfold;
   intros; try solve [eexists; eauto|congruence].
 
 Program Definition null_extension := Extension.Make 
-  wsem cores signature (null_extsig _ _ (ext_spec_type signature)) 
+  csem cores client_sig client_sig handled
   proj_core _
   active _ _
-  runnable _ _ _ _
-  proj_ext_state lift_pred _ _ _
-  inj_ext_state _ _.
+  runnable _ _ _ _ _ _
+  proj_zint proj_zext zmult _ _ _.
 Next Obligation.
 revert H0; case_eq (eq_nat_dec i 1).
-intros -> _; exists (snd w); auto.
+intros -> _; exists s; auto.
 congruence.
 Qed.
 Next Obligation.
-if_tac; exists (snd w); auto.
+if_tac; exists s; auto.
 elimtype False; apply H; auto.
 Qed.
 Next Obligation. 
-destruct (at_external csem (snd w)); try solve[congruence]. 
-destruct (safely_halted csem ge (snd w)); try solve[congruence].
+destruct (at_external csem s); try solve[congruence]. 
+destruct (safely_halted csem ge s); try solve[congruence].
 Qed.
 Next Obligation. 
-case_eq (at_external csem (snd w)); try solve[congruence]. 
+case_eq (at_external csem s); try solve[congruence]. 
 intros [ef args] H2.
 rewrite H2 in H; right; exists ef; exists args.
 inversion H0; subst; auto.
 inversion H1; subst; auto.
 intros H2; rewrite H2 in H.
-case_eq (safely_halted csem ge (snd w)). 
+case_eq (safely_halted csem ge s). 
 intros rv H3; left; exists rv.
 inversion H0; subst.
 inversion H1; subst.
@@ -136,47 +96,41 @@ congruence.
 Qed.
 Next Obligation. inversion H; subst; eapply after_at_external_excl; eauto. Qed.
 Next Obligation. inversion H; subst; eapply at_external_handled; eauto. Qed.
-Next Obligation. destruct w; destruct w'; simpl in *; destruct H; auto. Qed.
-Next Obligation. apply null_extsig_linkable. Qed.
+Next Obligation. inversion H; subst; if_tac in H0; try congruence. Qed.
+Next Obligation. unfold linkable; intros; inv H0; inv H1; exists x'; auto. Qed.
 
-Section NullExtensionSafe.
-Variable (csem_det: forall ge c m c' m' c'' m'',
-           corestep csem ge c m c' m' -> corestep csem ge c m c'' m'' -> 
-           (c', m')=(c'', m'')).
-
-Lemma null_extension_safe : safe_extension null_extension.
+Lemma null_extension_safe (csem_fun: corestep_fun csem) : 
+  safe_extension null_extension.
 Proof.
 apply safety_criteria_safe; constructor; autounfold with null_unfold in *.
 
 (*1*) intros until m'; intros H1 H2 [H3 H4] H5 H6. 
-split; auto. split; auto. inversion H6; subst; simpl.
-autounfold with null_unfold in *.
-inversion H3; rewrite H7 in *.
-inversion H4; rewrite H8 in *.
-f_equal; generalize (csem_det _ _ _ _ _ _ _ H H5); inversion 1; auto.
-inversion H6; subst.
-unfold Extension.all_safe; intros i CS0 c0; inversion 1.
-rewrite H8 in *.
-intros H9; simpl in H4; autounfold with null_unfold in *; simpl in *.
-autounfold with null_unfold in *.
-inversion H4; rewrite H10 in *.
-inversion H9; rewrite H11 in *.
-if_tac in H11; try solve[congruence].
-inversion H11; rewrite H13 in *.
+inversion H3 as [H7]; rewrite <-H7 in *; clear H7 H3.
+unfold Extension.proj_core in H4; simpl in H4.
+generalize H4 as H4'; intro.
+unfold proj_core in H4; if_tac in H4; try solve[congruence].
+inversion H4 as [H7]; rewrite H7 in *; clear H7 H4.
+rewrite H in *; clear H.
+split; auto.
+split; auto.
+unfold Extension.proj_core; simpl; unfold proj_core.
+if_tac; try solve[congruence].
+f_equal; generalize (csem_fun _ _ _ _ _ _ _ H5 H6); inversion 1; auto.
+simpl in H1|-*.
+unfold proj_zint, Extension.all_safe in *.
+intros until c0; intros H H8.
+inversion H as [H7]; rewrite H7 in *; clear H.
+unfold Extension.proj_core in H8; simpl in H8; unfold proj_core in H8.
+if_tac in H8; try solve[congruence].
+rewrite <-H in *; clear H; inversion H8 as [H].
+rewrite H in *; clear H8 H.
 eapply safe_corestep_forward; eauto.
-unfold corestep_fun; intros; eapply csem_det; eauto.
-specialize (H1 1 CS0 (snd w)); unfold proj_ext_state in H1.
-rewrite <-H0.
-assert (Extension.proj_ext_state null_extension w = fst w).
- simpl; autounfold with null_unfold; auto.
-rewrite <-H10, <-H12; apply H1; auto.
 
 (*2*) intros until CS; intros H1 H2 H3 [H4 H5].
 spec H1 i CS c H4 H5.
 simpl in H3.
-destruct w.
 unfold runnable in H3; simpl in H3.
-case_eq (at_external csem c0).
+case_eq (at_external csem s).
 intros [ef args] H6.
 rewrite H6 in H3.
 simpl in H5; unfold proj_core in H5; simpl in H5; inversion H5; subst.
@@ -192,33 +146,20 @@ rewrite H2 in H1.
 rewrite <-H7 in H1.
 destruct (safely_halted csem ge c); try solve[congruence].
 destruct H1 as [c' [m' [H8 H9]]].
-exists c'; exists (e, c'); exists m'; split; auto.
+exists c'; exists c'; exists m'; split; auto.
 rewrite <-H7; auto.
-split; auto.
-simpl.
-split; auto.
 
 (*3*) intros until x; intros [H1 H2] H3 H4 H5 H6 H7 H8.
-simpl in H6; unfold lift_pred in H6.
-generalize (Extension.csem_wsem_linkable null_extension); intros [H9 H10].
-simpl in H10.
-specialize (H10 ef x x).
-specialize (H10 (ext_spec_pre (null_extsig M extension_state 
-  (ext_spec_type signature)) ef x)).
-specialize (H10 (ext_spec_post (null_extsig M extension_state
-  (ext_spec_type signature)) ef x)).
-specialize (H10 P Q).
-spec H10; auto.
-spec H10; auto.
-destruct H10 as [H10 H11].
-specialize (H10 (sig_args sig) args w m H6); elimtype False; auto.
+apply ListSet.set_mem_correct1 in H4.
+unfold handled, ListSet.set_In in H4.
+inversion H4.
 
 (*4*) intros until m; intros H1 H2 H3.
 simpl in H2; unfold runnable in H2.
 inversion H3; subst.
 unfold compose in H0;  simpl in H0.
 rewrite H0 in H2.
-case_eq (safely_halted csem ge (snd w)); intros; try solve[congruence].
+case_eq (safely_halted csem ge s); intros; try solve[congruence].
 rewrite H in H2.
 right; exists i; auto.
 rewrite H in H2; congruence.
@@ -226,12 +167,11 @@ rewrite H in H2; congruence.
 (*5*) intros until rv; intros [H1 H2] H3 H4.
 split; auto.
 simpl.
-inversion H4; subst.
-apply corestep_not_halted in H.
+apply corestep_not_halted in H4.
 simpl in H2; inversion H2; subst.
-inversion H1; rewrite H7 in *.
-unfold proj_core in H6.
-if_tac in H6; try solve[congruence].
+inversion H1; rewrite H5 in *.
+unfold proj_core in H0.
+if_tac in H0; try solve[congruence].
 
 (*6*) intros until CS; inversion 1; subst.
 intros H4 H5; intros until j; intros H6; split.
@@ -241,7 +181,7 @@ simpl in H8; unfold proj_core in H8; simpl in H8; inversion H8; subst.
 simpl; unfold proj_core; simpl.
 simpl in H6; unfold active in H6.
 if_tac; auto; exfalso; apply H6; auto.
-intros n [H7 H8].
+intros n z z' [H7 H8].
 simpl in H8; unfold proj_core in H8; simpl in H8.
 simpl in H6; unfold active in H6; simpl in H6.
 if_tac in H8; auto.
@@ -250,23 +190,15 @@ exfalso; apply H6; auto.
 congruence.
 
 (*7*) intros until args; intros H1.
-exists csem; exists (snd w); split; auto.
+exists csem; exists s; split; auto.
 
-(*8*) intros until x.
+(*8*) intros until Q.
 intros [H1 H2] H3 H4 H5 H6.
-generalize (Extension.csem_wsem_linkable null_extension); intros [_ H10].
-specialize (H10 ef x x).
-specialize (H10 (ext_spec_pre (null_extsig M extension_state 
-  (ext_spec_type signature)) ef x)).
-specialize (H10 (ext_spec_post (null_extsig M extension_state
-  (ext_spec_type signature)) ef x)).
-specialize (H10 P Q).
-spec H10; auto.
-spec H10; auto.
-destruct H10 as [H10 H11].
-specialize (H10 tys args w m H4); elimtype False; auto.
+intros H12; simpl; exists c'; split3; auto.
+simpl in H2; unfold proj_core in H2.
+if_tac in H2; try solve[congruence].
 
-(*9*) intros until x; intros [H1 H2] H3 H4 H5 H6 H7 [H8 H9]; 
+(*9*) intros until Q; intros [H1 H2] H3 H4 H5 H6 H7 [H8 H9]; 
  intros until j; intros H10; split.
 intros [H11 H12].
 simpl in H12; unfold proj_core in H12; simpl in H12.
@@ -282,7 +214,5 @@ if_tac in H12.
 rewrite H in H10; exfalso; auto.
 congruence.
 Qed.
-
-End NullExtensionSafe.
 
 End NullExtension.
